Update JoinedView

src/sequential/ReorderFuture.v
@@ -34,14 +34,204 @@ Require Import gSimAux.
 
 Set Implicit Arguments.
 
+Inductive joined_promise_steps lang:
+  forall (th0 th1: Thread.t lang) (views0 views1: Loc.t -> Time.t -> list View.t), Prop :=
+| joined_promise_steps_base
+    th0 views0
+  :
+    joined_promise_steps th0 th0 views0 views0
+| joined_promise_steps_step
+    th0 th1 th2 views0 views1 views2
+    pf loc from to msg kind
+    (STEP: JThread.step pf (ThreadEvent.promise loc from to msg kind) th0 th1 views0 views1)
+    (STEPS: joined_promise_steps th1 th2 views1 views2)
+  :
+    joined_promise_steps th0 th2 views0 views2
+.
+
 Definition release_event (e: ThreadEvent.t): Prop :=
   match e with
   | ThreadEvent.update _ _ _ _ _ _ _ _ ordw => Ordering.le Ordering.strong_relaxed ordw
   | ThreadEvent.write _ _ _ _ _ ord => Ordering.le Ordering.strong_relaxed ord
   | ThreadEvent.fence _ ordw => Ordering.le Ordering.strong_relaxed ordw
   | ThreadEvent.syscall _ => True
+  | ThreadEvent.failure => True
+  | ThreadEvent.racy_write _ _ _ => True
+  | ThreadEvent.racy_update _ _ _ _ _ => True
   | _ => False
   end.
+
+Variant lower_step {lang} (th0 th1: Thread.t lang): Prop :=
+| lower_step_intro
+    pf e
+    (STEP: Thread.step pf e th0 th1)
+    (NPROMISE: no_promise e)
+    (NRELEASE: ~ release_event e)
+    (MEM: lower_memory th1.(Thread.memory) th0.(Thread.memory))
+.
+
+Variant lower_steps {lang} (th0 th1: Thread.t lang): Prop :=
+| lower_steps_intro
+    (STEPS: rtc (tau (@pred_step (fun e => no_promise e /\ ~ release_event e) lang)) th0 th1)
+    (MEM: lower_memory th1.(Thread.memory) th0.(Thread.memory))
+.
+
+Lemma lower_steps_equiv lang (th0 th1: Thread.t lang)
+  :
+    lower_steps th0 th1 <-> rtc lower_step th0 th1.
+Proof.
+  split.
+  { i. inv H. revert MEM. induction STEPS.
+    { i. refl. }
+    { i. admit. }
+  }
+  { i. induction H.
+    { econs; eauto. refl. }
+    { inv IHclos_refl_trans_1n. inv H. econs.
+      { econs; [|eauto]. econs.
+        { econs; eauto. econs; eauto. }
+        { destruct e; ss. }
+      }
+      { etrans; eauto. }
+    }
+  }
+Admitted.
+
+Definition delayed {lang} (th0 th1: Thread.t lang): Prop
+  :=
+    exists th1',
+      (<<STEPS: rtc (tau (@pred_step (fun e => no_promise e /\ ~ release_event e) lang)) th0 th1'>>) /\
+      (<<MEM: lower_memory th1'.(Thread.memory) th1.(Thread.memory)>>) /\
+      (<<SC: TimeMap.le th1'.(Thread.sc) th1.(Thread.sc)>>) /\
+      (<<STATE: th1'.(Thread.state) = th1.(Thread.state)>>) /\
+      (<<LOCAL: lower_local th1'.(Thread.local) th1.(Thread.local)>>).
+
+Lemma delayed_refl lang (th: Thread.t lang)
+  :
+    delayed th th.
+Proof.
+  eexists. esplits; eauto; try refl.
+Qed.
+
+Lemma step_split lang (th0 th2: Thread.t lang) pf e views0 views2
+      (STEP: JThread.step pf e th0 th2 views0 views2)
+      (NRELEASE: ~ release_event e)
+  :
+    exists th1,
+      (<<PROMISES: joined_promise_steps th0 th1 views0 views2>>) /\
+      (<<LOWER: rtc lower_step th1 th2>>) /\
+      (<<MEM: th1.(Thread.memory) = th2.(Thread.memory)>>) /\
+      (<<SC: th1.(Thread.sc) = th2.(Thread.sc)>>).
+Proof.
+  inv STEP. inv STEP0.
+  { inv STEP. esplits.
+    { econs; [|econs]. econs; eauto.
+      { econs. econs; eauto. }
+    }
+    { econs. }
+    { ss. }
+    { ss. }
+  }
+  { inv STEP. inv LOCAL; ss.
+    { esplits.
+      { econs; [|econs]
+        {
+
+
+      { eauto. }
+
+        eauto.  ss. econs.
+
+        econs.
+        {
+
+
+  /\
+
+
+      /\
+
+      (<<STEP: Thread.step pf th0 th2>>).
+
+
+
+
+destruct (Thread.local th); ss.
+
+
+
+
+        Thread.mk _ st0 lc0 sc1 mem1) (Thread.mk _ st1 lc1' sc1 mem1')>>) /\
+      (<<LOCAL: lower_local lc1' lc1>>) /\
+      (<<MEM: lower_memory mem1' mem1>>).
+
+
+      lang (st0 st1: Language.state lang) (lc0 lc1: Local.t)
+           (mem0: Memory.t)
+           (sc0: TimeMap.t)
+           (views0: Loc.t -> Time.t -> list View.t)
+           (fin: Messages.t): Prop
+  :=
+    forall (mem1: Memory.t)
+           (sc1: TimeMap.t)
+           (views1: Loc.t -> Time.t -> list View.t)
+           (MEM: Memory.closed mem1)
+           (FUTURE: Memory.future mem0 mem1)
+           (SCLE: TimeMap.le sc0 sc1)
+           (FINALIZED: fin <4= Messages.of_memory mem1)
+           (VIEWLE: views_le views0 views1)
+           (VIEWS: wf_views views1)
+           (JOINED: joined_memory views1 mem1)
+           (SC: Memory.closed_timemap sc1 mem1)
+           (LOCAL: Local.wf lc1 mem1),
+    exists mem1' lc1',
+      (<<LOCAL: Local.wf lc0 mem1>>) /\
+      (<<JOINED: joined_released views1 lc0.(Local.promises) lc0.(Local.tview).(TView.rel)>>) /\
+      (<<STEPS: rtc (tau (@pred_step (fun e => no_promise e /\ ~ release_event e) lang)) (Thread.mk _ st0 lc0 sc1 mem1) (Thread.mk _ st1 lc1' sc1 mem1')>>) /\
+      (<<LOCAL: lower_local lc1' lc1>>) /\
+      (<<MEM: lower_memory mem1' mem1>>)
+.
+
+Lemma delayed_current
+      lang (st: Language.state lang) lc
+      mem0 sc0 views0 fin
+  :
+    delayed _ st st lc lc mem0 sc0 views0 fin.
+Proof.
+Admitted.
+
+Lemma delayed_future
+      lang (st0 st1: Language.state lang) lc0 lc1
+      mem0 sc0 views0 fin0
+      mem1 sc1 views1 fin1
+      (MEM: Memory.future mem0 mem1)
+      (SC: TimeMap.le sc0 sc1)
+      (VIEWS: views_le views0 views1)
+      (FIN: fin0 <4= fin1)
+      (FINALIZED: fin1 <4= Messages.of_memory mem1)
+      (DELAYED: delayed _ st0 st1 lc0 lc1 mem0 sc0 views0 fin0)
+  :
+    delayed _ st0 st1 lc0 lc1 mem1 sc1 views1 fin1.
+Proof.
+Admitted.
+
+Lemma delayed_step
+      lang (st0 st1 st2: Language.state lang) lc0 lc1 lc2
+      mem1 sc1 views1 mem2 sc2 views2 fin
+      pf e
+      (STEP: JThread.step pf e (Thread.mk _ st1 lc1 sc1 mem1) (Thread.mk _ st2 lc2 sc2 mem2) views1 views2)
+      (NRELEASE: ~ release_event e)
+      (DELAYED: delayed _ st0 st1 lc0 lc1 mem1 sc1 views1 fin)
+  :
+    exists lc0',
+      (<<PROMISES: joined_promise_steps (Thread.mk _ st0 lc0 sc1 mem1) (Thread.mk _ st0 lc0' sc2 mem2) views1 views2>>) /\
+      (<<DELAYED: delayed _ st0 st2 lc0' lc2 mem2 sc2 views2 (fin \4/ committed mem1 lc1.(Local.promises) mem2 lc2.(Local.promises))>>).
+Proof.
+Admitted.
+
+
+
+
 
 Definition delayed
            lang (st0 st1: Language.state lang) (lc0 lc1: Local.t)
@@ -70,73 +260,39 @@ Definition delayed
       (<<MEM: lower_memory mem1' mem1>>)
 .
 
-(* Lemma delayed_future *)
-(*       lang (st0 st1: Language.state lang) lc0 lc1 *)
-(*       mem0 sc0 views0 fin *)
-(*       (DELAYED: delayed st0 st1 lc0 lc1 mem0 sc0 views0 fin) *)
-(*       mem1 sc1 views1 *)
-(*       (MEM: Memory.closed mem1) *)
+Lemma delayed_current
+      lang (st: Language.state lang) lc
+      mem0 sc0 views0 fin
+  :
+    delayed _ st st lc lc mem0 sc0 views0 fin.
+Proof.
+Admitted.
 
+Lemma delayed_future
+      lang (st0 st1: Language.state lang) lc0 lc1
+      mem0 sc0 views0 fin0
+      mem1 sc1 views1 fin1
+      (MEM: Memory.future mem0 mem1)
+      (SC: TimeMap.le sc0 sc1)
+      (VIEWS: views_le views0 views1)
+      (FIN: fin0 <4= fin1)
+      (FINALIZED: fin1 <4= Messages.of_memory mem1)
+      (DELAYED: delayed _ st0 st1 lc0 lc1 mem0 sc0 views0 fin0)
+  :
+    delayed _ st0 st1 lc0 lc1 mem1 sc1 views1 fin1.
+Proof.
+Admitted.
 
-(*            (MEM: Memory.closed mem1) *)
-(*            (FUTURE: Memory.future mem0 mem1) *)
-(*            (SCLE: TimeMap.le sc0 sc1) *)
-(*            (FINALIZED: fin <4= Messages.of_memory mem1) *)
-(*            (VIEWLE: views_le views0 views1) *)
-(*            (VIEWS: wf_views views1) *)
-(*            (JOINED: joined_memory views1 mem1) *)
-(*            (SC: Memory.closed_timemap sc1 mem1) *)
-(*            (LOCAL: Local.wf lc1 mem1), *)
-
-
-(*       (SC: *)
-
-(* Lemma step_delayed *)
-(*       lang st0 st1 st2 lc0 lc1 lc2 *)
-(*       mem1 views0 views1 fin0 *)
-(*       pf e *)
-(*       (STEP: JThread.step pf e (Thread.mk _ st1 lc1 sc1 mem1) (Thread.mk _ st2 lc2 sc2 mem2)) *)
-(*       (SILENT: no_promise e) *)
-(*       (DELAYED: delayed st0 st1 lc0 lc1 mem- m *)
-(*   : *)
-(*     exists pf' e' st0' lc0', *)
-(*       (<<STEP: JThread.opt_step pf' e' *)
-
-
-
-(*       (st0 st1: Language.state lang) (lc0 lc1: Local.t) *)
-(*       (mem0: Memory.t) *)
-
-
-(* Definition delayed_strong *)
-(*            lang (st0 st1: Language.state lang) (lc0 lc1: Local.t) *)
-(*            (mem0: Memory.t) *)
-(*            (sc0: TimeMap.t) *)
-(*            (views0: Loc.t -> Time.t -> list View.t) *)
-(*            (fin: Messages.t): Prop *)
-(*   := *)
-(*     forall (mem1: Memory.t) *)
-(*            (sc1: TimeMap.t) *)
-(*            (views1: Loc.t -> Time.t -> list View.t) *)
-(*            (MEM: Memory.closed mem1) *)
-(*            (FUTURE: Memory.future mem0 mem1) *)
-(*            (SCLE: TimeMap.le sc0 sc1) *)
-(*            (FINALIZED: fin <4= Messages.of_memory mem1) *)
-(*            (VIEWLE: views_le views0 views1) *)
-(*            (VIEWS: wf_views views1) *)
-(*            (JOINED: joined_memory views1 mem1) *)
-(*            (SC: Memory.closed_timemap sc1 mem1) *)
-(*            (LOCAL: Local.wf lc1 mem1) *)
-
-(*            (lc0': Local.t) *)
-(*            (TVIEW: TView.le lc1'.(Local.tview) lc1.(Local.tview)) *)
-
-
-(*     , *)
-(*     exists mem1' lc1', *)
-(*       (<<LOCAL: Local.wf lc0 mem1>>) /\ *)
-(*       (<<JOINED: joined_released views1 lc0.(Local.promises) lc0.(Local.tview).(TView.rel)>>) /\ *)
-(*       (<<STEPS: rtc (tau (@pred_step (fun e => no_promise e /\ ~ release_event e) lang)) (Thread.mk _ st0 lc0 sc1 mem1) (Thread.mk _ st1 lc1' sc1 mem1')>>) /\ *)
-(*       (<<TVIEW: TView.le lc1'.(Local.tview) lc1.(Local.tview)>>) /\ *)
-(*       (<<PROMISES: lc1'.(Local.promises) = lc1.(Local.promises)>>) *)
-(* . *)
+Lemma delayed_step
+      lang (st0 st1 st2: Language.state lang) lc0 lc1 lc2
+      mem1 sc1 views1 mem2 sc2 views2 fin
+      pf e
+      (STEP: JThread.step pf e (Thread.mk _ st1 lc1 sc1 mem1) (Thread.mk _ st2 lc2 sc2 mem2) views1 views2)
+      (NRELEASE: ~ release_event e)
+      (DELAYED: delayed _ st0 st1 lc0 lc1 mem1 sc1 views1 fin)
+  :
+    exists lc0',
+      (<<PROMISES: joined_promise_steps (Thread.mk _ st0 lc0 sc1 mem1) (Thread.mk _ st0 lc0' sc2 mem2) views1 views2>>) /\
+      (<<DELAYED: delayed _ st0 st2 lc0' lc2 mem2 sc2 views2 (fin \4/ committed mem1 lc1.(Local.promises) mem2 lc2.(Local.promises))>>).
+Proof.
+Admitted.
